% ---------
%  Compile with "pdflatex hw0".
% --------
%!TEX TS-program = pdflatex
%!TEX encoding = UTF-8 Unicode

\documentclass[11pt]{article}
\usepackage{jeffe,handout,graphicx}
\usepackage[utf8]{inputenc}     % Allow some non-ASCII Unicode in source
\usepackage{amsmath}
\usepackage{listings}
\usepackage{tikz}

%  Redefine suits
\usepackage{pifont}
\def\Spade{\text{\ding{171}}}
\def\Heart{\text{\textcolor{Red}{\ding{170}}}}
\def\Diamond{\text{\textcolor{Red}{\ding{169}}}}
\def\Club{\text{\ding{168}}}

\def\Cdot{\mathbin{\text{\normalfont \textbullet}}}
\def\Sym#1{\textbf{\texttt{\color{BrickRed}#1}}}
\let\oriinfty=\infty
\def\infty{{\oriinfty\llap{\vrule height.24em depth-.2em width.2em}}}

%%% magic code starts
\mathcode`*=\string"8000
\begingroup
\catcode`*=\active
\xdef*{\noexpand\textup{\string*}}
\endgroup
%%% magic code ends
%%% check mark
\def\checkmark{\tikz\fill[scale=0.4](0,.35) -- (.25,0) -- (1,.7) -- (.25,.15) -- cycle;}

% =====================================================
%   Define common stuff for solution headers
% =====================================================
\Class{Abstract Algebra}
\Semester{}
\Authors{1}
\AuthorOne{Aneesh Durg}
%\Section{}

% =====================================================
\begin{document}
% Copy this section again for a new solution
% ---------------------------------------------------------
\ExerciseHeader{4}{4} % replace Chapter with Exercise for a different header
\begin{itemize}
    \item[1)] 
    \vspace{6pt}
    \hrule
    \vspace{6pt}
    \item[2)] 
    \vspace{6pt}
    \hrule
    \vspace{6pt}
    \item[8)]
    \vspace{6pt}
    \hrule
    \vspace{6pt}
    \item[24)]
    \begin{solution}\hfill \\
        We just need to show that for any $(ab)$, we can construct it from the allowed transpositions. This is because any permutation can be built from transpositions.
        \begin{itemize}
            \item[a)]
                $$(ab) = (1a)(1a)(ab) = (1a)(1ab) = (1a)(b1a) = (1a)(b1)(1a) = (1a)(1b)(1a)$$
            \item[b)]
                b:
                (ab) = (aa')(aa')(ab) = (aa')(a'ab) = (aa')(a'ab)(bb')(bb')
            \item[c)]\\
                Show that we can get $(a a-1)$ for any $a$ from $(12...n) \forall n$ and then use part $b$. We also know that:
                $$(a_1 \dots a_nb)(bc) = (a_1\dots a_nbc)$$
                Using this:
                $$(12)(123) = (12)(12)(23) = (23)$$
                $$(12)(123)(12)(1234) = (23)(12)(123)(34) = (34)$$
                can inductively generate any $(a a-1)$
        \end{itemize}
    \end{solution}
    \vspace{6pt}
    \hrule
    \vspace{6pt}
\end{itemize}
\vspace{6pt}
\hrule
\vspace{6pt}
% ---------------------------------------------------------
\end{document}

